\documentclass[12pt]{amsart}
\usepackage[left=0.5in, right=0.5in, bottom=0.75in, top=0.75in]{geometry}
\usepackage[english]{babel}
\usepackage[utf8x]{inputenc}
\usepackage{amsmath,amssymb,amsthm}
\usepackage{enumerate}
\usepackage{graphicx}

\begin{document}
\raggedbottom

\noindent{\large OPER 610 - Linear Programming %
	% Lesson X %
	(Due Feb 28 at 10am)}
\hspace{\fill} {\large B. Hosley}
\bigskip


%%%%%%%%%%%%%%%%%%%%%%%
\setcounter{section}{8}
\setcounter{subsection}{0}
\subsection{}
Solve the problem to minimize  \(3x_1 + 2x_2\), subject to \(x_1 + 2x_2 \geq 2\) and \(x_1 \geq 0\), 
\(x_2 \geq 0\), using Karmarkar's algorithm by equivalently transforming the problem into 
the form (8.4) that satisfies Assumptions (A1) and (A2). Plot the iterates you 
generate in the \(( x_1 ,x_2 )\) space.

\bigskip
\textbf{Solution:}

Due to the unfortunate \(\geq2\) we must convert the system into something else to meet 
assumptions A1 and A2.

First, we determine that the dual of the original problem is
to maximize \(2w_1\) subject to \(w_1\leq3\), \(2w_1\leq2\), and \(w_1\geq0\).
We can eliminate \(w_1\leq3\) as a redundant constraint.
Then, we add slack variables;
\begin{align*}
	x_1 + 2x_2 - x_3 &= 2 & 2w_1 + w_2 &= 2 \\
	3x_1 + 2x_2 &= 2w_1 & \mathbf{x}, \mathbf{w} &\geq \mathbf{0}.
\end{align*}
Next we add a bounding constraint \(Q\) and corresponding slack variables, 
wherein it is assumed that \(s_2=1\);
\begin{align*}
	x_1 + 2x_2 - x_3 - 2s_2 &= 0 & 2w_1 + w_2 -2s_2 &= 0 \\
	3x_1 + 2x_2 - 2w_1 &= 0   \\
	\sum_{i}x_i + \sum_{i}w_i + s_1 - Qs_2 &= 0 & \sum_{i}x_i+\sum_{i}w_i + s_1 + s_2 &= Q-1 \\
	\mathbf{x}, \mathbf{w}, \mathbf{s} &\geq \mathbf{0}.
\end{align*}
Next we use a variable change to get,
\begin{align*}
	y_1 + 2y_2 - y_3 - 2y_7 &= 0 & 2y_4 + y_5 -2y_7 &= 0 \\
	3y_1 + 2y_2 - 2y_4 &= 0   \\
	\sum_i^6y_i - Qy_7 &= 0 & \sum_{i}^7y_i &= 1 \\
	\mathbf{y} &\geq 0.
\end{align*}
Which is equivalent to 
\begin{alignat*}{8}
	\min\quad\,\ y_8 \\
	\text{subject to}\quad\,\ 
	 y_1& {}+{} & 2x_2& {}-{} & y_3 &  { }  &  {}  &  { }  & {}  & {}-{} & 2y_7 &  { }  & {}  & {}={} & 0 \\
	 {} &  { }  &  {} &  { }  & {}  &  { }  & 2y_4 & {}+{} & y_5 & {}-{} & y_7  & {}-{} & 2y_8& {}={} & 0 \\
	3y_1& {}+{} & 2y_2&  { }  & {}  & {}-{} & 2y_4 &  { }  & {}  &  { }  & {}   & {}-{} & 3y_8& {}={} & 0 
\end{alignat*}
\[ \hspace{25ex} \sum_i^6y_i - Qy_7 + (Q-5)y_8  {}={} 0 \]
\[ \hspace{30ex} \sum_i^8y_i = 1,\quad \text{and} \quad \mathbf{y} \geq \mathbf{0} .\]

This equation satisfies assumptions A1 and A2.


\end{document}