\section{Transformations and Expectations}
	\begin{equation*}
		E_g(X) = 
		\begin{cases}
			\sum_{x\in\mathcal X} g(x)f_X(x) & \text{discrete} \\
			\int_{-\infty}^{\infty} g(x)f_X(x) \,dx & \text{continuous}
		\end{cases}
	\end{equation*}
	
	\subsection*{Properties of Expectations}
		\begin{enumerate}
			\item \(E[ag_1(X) +bg_2(X) + c] \)\\ \(= aE_{g1}[X] + bE_{g2}[X] + c \)
			\item If \(g_1(x)\geq0\) for all \(x\), \\ then \(E_{g1}[X]\geq0\)
			\item If \(g_1(x) \geq g_2(x)\) for all \(x\), \\ then \(E_{g_1}[X] \geq E_{g_2}[X]\)
			\item If \(a \leq g_1(X) \leq b\) for all \(x\), \\ then \(a \leq E_{g_1}[X] \leq b\)
			\item (other properties) \(E[k] = k\)
			\item \(E[(X-b)^2]\) is a min for \(b=E[X]\)
		\end{enumerate}
		
	\subsection{CDF Transform}
		If \(X\) is a continuous random variable
		\begin{equation*}
			F_Y(y) = \begin{cases}
				F_X(g^{-1}(y)) & g\ \text{\scriptsize increasing on }X \\
				1- F_X(g^{-1}(y)) & g\ \text{\scriptsize decreasing on }X
			\end{cases}
		\end{equation*}
		
	\subsection{Univariate Transform}
		\begin{equation*}
			f_Y(y) = \begin{cases}
				\int_{-\infty}^{\infty} f_x(g^{-1}(y))|\frac{d}{dy}g^{-1}(y)| & y \in \mathcal{Y} \\
				\sum_{i=1}^{k} f_x(g^{-1}(y)) & y \in \mathbb{Z}\\
				0 & else
			\end{cases}
		\end{equation*}
	
	\subsection*{Iterated Expectations}
		\begin{equation*}
			\begin{split}
				E[g(y)|x]  
				&= \sum_{n} g(y)f_{Y|X}(x|y) \\
				&= \int_{\mathbb{R}} g(y)f_{Y|X}(y|x) 
			\end{split}
		\end{equation*}
		\[E[X] = E_Y[E_X[X|Y]]\]
		\[\text{Var}[X] = E_Y[\text{Var}_X[X|Y]] + \text{Var}_Y[E_X[X|Y]]\]
		
	\subsection*{Moments}
		\subsubsection*{Moment Generating Function}
			\begin{equation*}
				\begin{split}
					m_x(t) &= E[e^{tx}] \\
					&= \sum_{x\in\mathcal X} e^{tx}\,f_X(x) \\
					&= 1 + E[X] + \ldots + \frac{t^nE[X^n]}{n!} \\
					&= \int_{-\infty}^{\infty} e^{tx} f_X(x) \,dx
				\end{split}
			\end{equation*}
			Let \(Z=X+Y\)
			\[M_Z(t) = M_X(t)M_Y(t)\]
	
	\subsection*{Leibnitz's Rule}
		\begin{equation*}
			\begin{split}
				\frac{d}{d\theta} 
				\int^{b(\theta)}_{a(\theta)} f(x, \theta) \,dx
				&= f(b(\theta), \theta) \frac{d}{d\theta} b(\theta) \\
				- f(a(\theta), \theta) \frac{d}{d\theta} a(\theta)
				&+  \int^{b(\theta)}_{a(\theta)}\frac{\partial}{\partial\theta} f(x, \theta) \,dx
			\end{split}
		\end{equation*}
	
